all2.v
@@ -69,7 +69,6 @@ Proof. formula_induction A. Qed.
 Hint Rewrite fup_fup_com : term_db.
 
 
-
 (** substitutes [formula] [F] for variable [X] in [formula] [A] (capture is possible) *)
 Fixpoint subs X F A :=
 match A with
@@ -78,7 +77,7 @@ match A with
 | cst R => cst R
 | top => top
 | wdg B C => wdg (subs X F B) (subs X F C)
-| frl Y B as C => if (eqb Y X) then C else frl Y (subs X F B)
+| frl Y B => frl Y (if (eqb Y X) then B else subs X F B)
 end.
 
 Lemma fsize_subs_dvar : forall k X A, fsize (subs X (dvar k) A) = fsize A.
